reflection: show collect_app/mk_app are inverses
one way only, missing the other, trickier, one

ulib/FStar.Reflection.Formula.fst
@@ -40,7 +40,29 @@ let rec mk_app (t : term) (args : list term) : Tot term (decreases args) =
     | [] -> t
     | (x::xs) -> mk_app (pack (Tv_App t x)) xs
 
-(* We could prove the previous two functions are inverses given some specs about pack/inspect *)
+val uncurry : ('a -> 'b -> 'c) -> ('a * 'b -> 'c)
+let uncurry f (x, y) = f x y
+
+val curry : ('a * 'b -> 'c) -> ('a -> 'b -> 'c)
+let curry f x y = f (x, y)
+
+val mk_app_collect_inv_s : (t:term) -> (args:list term) ->
+                            Lemma (uncurry mk_app (collect_app' args t) == mk_app t args)
+let rec mk_app_collect_inv_s t args =
+    match inspect t with
+    | Tv_App l r ->
+        mk_app_collect_inv_s l (r::args);
+        pack_inspect_inv t
+    | _ -> ()
+
+val mk_app_collect_inv : (t:term) -> Lemma (uncurry mk_app (collect_app t) == t)
+let rec mk_app_collect_inv t = mk_app_collect_inv_s t []
+
+(*
+ * The way back is not stricly true: the list of arguments could grow.
+ * It's annoying to even state, might do it later
+ *)
+
 let term_view_as_formula (tv:term_view) : Tot formula =
     match tv with
     | Tv_Var n ->
